src/lowparse/LowParse.Spec.DER.fst
@@ -1,0 +1,133 @@
+module LowParse.Spec.DER
+include LowParse.Spec.Combinators
+include LowParse.Spec.Bytes
+
+include LowParse.Spec.Int
+open FStar.Mul
+
+module B32 = FStar.Bytes
+module U8 = FStar.UInt8
+module UInt = FStar.UInt
+module Math = LowParse.Math
+module E = LowParse.BigEndian
+
+#reset-options "--z3cliopt smt.arith.nl=false --max_fuel 0 --max_ifuel 0"
+
+let der_length_max : nat = normalize_term (pow2 (8 * 126) - 1)
+
+let _ = intro_ambient der_length_max
+
+let _ : unit = _ by (FStar.Tactics.(print (string_of_int der_length_max); exact (`())))
+
+let der_length_t = (x: nat { x <= der_length_max })
+
+inline_for_extraction
+let parse_der_length_payload_kind : parser_kind = strong_parser_kind 0 126 None
+
+let rec log256
+  (x: nat { x > 0 })
+: GTot (y: nat { y > 0 /\ pow2 (8 * (y - 1)) <= x /\ x < pow2 (8 * y)})
+= assert_norm (pow2 8 == 256);
+  if x < 256
+  then 1
+  else begin
+    let n = log256 (x / 256) in
+    Math.pow2_plus (8 * (n - 1)) 8;
+    Math.pow2_plus (8 * n) 8;
+    n + 1
+  end
+
+let log256_unique
+  (x: nat)
+  (y: nat)
+: Lemma
+  (requires (
+    x > 0 /\
+    y > 0 /\
+    pow2 (8 * (y - 1)) <= x /\
+    x < pow2 (8 * y)
+  ))
+  (ensures (y == log256 x))
+= Math.pow2_lt_recip (8 * (y - 1)) (8 * log256 x);
+  Math.pow2_lt_recip (8 * (log256 x - 1)) (8 * y)
+
+let tag_of_der_length
+  (x: der_length_t)
+: GTot U8.t
+= if x < 128
+  then U8.uint_to_t x
+  else
+    let len_len = log256 x in
+    assert_norm (der_length_max == pow2 (8 * 126) - 1);
+    Math.pow2_lt_recip (8 * (len_len - 1)) (8 * 126);
+    128uy `U8.add` U8.uint_to_t len_len
+
+let synth_be_int
+  (len: nat)
+  (b: B32.lbytes len)
+: GTot (x: nat { x < pow2 (8 * len) })
+= E.lemma_be_to_n_is_bounded (B32.reveal b);
+  E.be_to_n (B32.reveal b)
+
+let synth_be_int_injective
+  (len: nat)
+: Lemma
+  (synth_injective (synth_be_int len))
+  [SMTPat (synth_injective (synth_be_int len))]
+= 
+  synth_injective_intro' (synth_be_int len) (fun (x x' : B32.lbytes len) ->
+    E.be_to_n_inj (B32.reveal x) (B32.reveal x')
+  )
+
+let parse_der_length_payload
+  (x: U8.t)
+: Tot (parser parse_der_length_payload_kind (refine_with_tag tag_of_der_length x))
+= assert_norm (der_length_max == pow2 (8 * 126) - 1);
+  assert_norm (pow2 7 == 128);
+  assert_norm (pow2 8 == 256);
+  assert_norm (256 < der_length_max);
+  assert (U8.v x <= der_length_max);
+  let (x' : der_length_t) = U8.v x in
+  if x' < 128
+  then begin
+    weaken parse_der_length_payload_kind (parse_ret (x' <: refine_with_tag tag_of_der_length x))
+  end else
+   if x = 128uy
+   then 
+    fail_parser parse_der_length_payload_kind (refine_with_tag tag_of_der_length x) // DER representation of 0 is covered by the x<128 case
+   else if x = 255uy
+   then 
+    fail_parser parse_der_length_payload_kind (refine_with_tag tag_of_der_length x) // forbidden in BER already
+   else if x = 129uy
+   then
+    weaken parse_der_length_payload_kind
+      ((parse_u8 `parse_filter` (fun y -> U8.v y >= 128))
+        `parse_synth` (fun (y: U8.t { U8.v y >= 128 } ) -> (
+          log256_unique (U8.v y) 1;
+          U8.v y <: refine_with_tag tag_of_der_length x
+      )))
+  else begin
+    let len = U8.v x % pow2 7 in
+    Math.lemma_mod_lt (U8.v x) (pow2 7);
+    Math.lemma_div_mod (U8.v x) (pow2 7);
+    Math.division_definition (U8.v x) (pow2 7) 1;
+    Math.pow2_le_compat (8 * 126) (8 * len);
+    Math.pow2_le_compat (8 * (len - 1)) 7;
+    synth_be_int_injective len;
+    weaken parse_der_length_payload_kind
+      (((parse_flbytes len `parse_synth` (synth_be_int len))
+        `parse_filter` (fun (y: nat { y < pow2 (8 * len) } ) -> y >= pow2 (8 * (len - 1))))
+       `parse_synth` (fun (y: (y: nat { y < pow2 (8 * len) } ) { y >= pow2 (8 * (len - 1)) } ) ->
+         log256_unique y len;
+         y <: refine_with_tag tag_of_der_length x
+      ))
+  end        
+        
+inline_for_extraction
+let parse_der_length_kind : parser_kind = and_then_kind parse_u8_kind parse_der_length_payload_kind
+
+let parse_der_length : parser parse_der_length_kind der_length_t
+= parse_tagged_union
+    parse_u8
+    tag_of_der_length
+    parse_der_length_payload
