src/lowparse/LowParse.Spec.fst
@@ -15,3 +15,4 @@ include LowParse.Spec.Option
 include LowParse.Spec.IfThenElse
 include LowParse.Spec.VCList
 include LowParse.Spec.BCVLI
+include LowParse.Spec.DER
